Weidenbach_Book/CDCL_Abstract_Clause_Representation.thy
@@ -1,0 +1,99 @@
+theory CDCL_Abstract_Clause_Representation
+imports Main Partial_Annotated_Clausal_Logic
+begin
+subsection \<open>Abstract Clause Representation\<close>
+text \<open>We will abstract the representation of clause and clauses via two locales. We expect our
+  representation to behave like multiset, but the internal representation can be done using list
+  or whatever other representation.\<close>
+locale raw_cls =
+  fixes
+    mset_cls:: "'cls \<Rightarrow> 'v clause" and
+    union_cls :: "'cls \<Rightarrow> 'cls \<Rightarrow> 'cls" and
+    insert_cls :: "'v literal \<Rightarrow> 'cls \<Rightarrow> 'cls" and
+    remove_lit :: "'v literal \<Rightarrow> 'cls \<Rightarrow> 'cls"
+  assumes
+    insert_cls[simp]: "mset_cls (insert_cls L C) = mset_cls C + {#L#}" and
+    mset_cls_union_cls[simp]: "mset_cls (union_cls C D) = mset_cls C #\<union> mset_cls D" and
+    remove_lit[simp]: "mset_cls (remove_lit L C) = remove1_mset L (mset_cls C)"
+begin
+end
+
+text \<open>This is a copy of the unnamed theorem of @{file "~~/src/HOL/Library/Multiset.thy"}.\<close>
+lemma union_mset_list:
+  "mset xs #\<union> mset ys =
+    mset (case_prod append (fold (\<lambda>x (ys, zs). (remove1 x ys, x # zs)) xs (ys, [])))"
+proof -
+  have "\<And>zs. mset (case_prod append (fold (\<lambda>x (ys, zs). (remove1 x ys, x # zs)) xs (ys, zs))) =
+      (mset xs #\<union> mset ys) + mset zs"
+    by (induct xs arbitrary: ys) (simp_all add: multiset_eq_iff)
+  then show ?thesis by simp
+qed
+
+text \<open>Instanciation of the previous locale, in an unnamed context to avoid polluating with simp
+  rules\<close>
+context
+begin
+  interpretation list_cls: raw_cls mset
+    "\<lambda>xs ys. case_prod append (fold (\<lambda>x (ys, zs). (remove1 x ys, x # zs)) xs (ys, []))"
+    "op #" remove1
+    by unfold_locales (auto simp: union_mset_list)
+
+  interpretation cls_cls: raw_cls id
+    "op #\<union>" "\<lambda>L C. C + {#L#}" remove1_mset
+    by unfold_locales (auto simp: union_mset_list)
+end
+
+locale raw_clss =
+  raw_cls mset_cls union_cls insert_cls remove_lit
+  for
+    mset_cls:: "'cls \<Rightarrow> 'v clause" and
+    union_cls :: "'cls \<Rightarrow> 'cls \<Rightarrow> 'cls" and
+    insert_cls :: "'v literal \<Rightarrow> 'cls \<Rightarrow> 'cls" and
+    remove_lit :: "'v literal \<Rightarrow> 'cls \<Rightarrow> 'cls" +
+  fixes
+    mset_clss:: "'clss \<Rightarrow> 'v clauses" and
+    union_clss :: "'clss \<Rightarrow> 'clss \<Rightarrow> 'clss" and
+    in_clss :: "'cls \<Rightarrow> 'clss \<Rightarrow> bool" and
+    insert_clss :: "'cls \<Rightarrow> 'clss \<Rightarrow> 'clss" and
+    remove_from_clss :: "'cls \<Rightarrow> 'clss \<Rightarrow> 'clss"
+  assumes
+    insert_clss[simp]: "mset_clss (insert_clss L C) = mset_clss C + {#mset_cls L#}" and
+    union_clss[simp]: "mset_clss (union_clss C D) = mset_clss C + mset_clss D" and
+    mset_clss_union_clss[simp]: "mset_clss (insert_clss C' D) = {#mset_cls C'#} + mset_clss D" and
+    in_clss_mset_clss[dest]: "in_clss a C \<Longrightarrow> mset_cls a \<in># mset_clss C" and
+    in_mset_clss_exists_preimage: "b \<in># mset_clss C \<Longrightarrow> \<exists>b'. in_clss b' C \<and> mset_cls b' = b" and
+    remove_from_clss_mset_clss[simp]:
+      "mset_clss (remove_from_clss a C) = mset_clss C - {#mset_cls a#}" and
+    in_clss_union_clss[simp]:
+      "in_clss a (union_clss C D) \<longleftrightarrow> in_clss a C \<or> in_clss a D"
+begin
+
+end
+
+experiment
+begin
+  fun remove_first where
+  "remove_first _ [] = []" |
+  "remove_first C (C' # L) = (if mset C = mset C' then L else C' # remove_first C L)"
+
+  lemma remove1_mset_single_add:
+    "a \<noteq> b \<Longrightarrow> remove1_mset a ({#b#} + C) = {#b#} + remove1_mset a C"
+    "remove1_mset a ({#a#} + C) = C"
+    by (auto simp: multiset_eq_iff)
+
+  lemma mset_map_mset_remove_first:
+    "mset (map mset (remove_first a C)) = remove1_mset (mset a) (mset (map mset C))"
+    by (induction C) (auto simp: ac_simps remove1_mset_single_add)
+
+  interpretation clss_clss: raw_clss id "op #\<union>" "\<lambda>L C. C + {#L#}" remove1_mset
+    id "op +" "op \<in>#" "\<lambda>L C. C + {#L#}" remove1_mset
+    by unfold_locales (auto simp: ac_simps)
+
+  interpretation list_clss: raw_clss mset
+    "\<lambda>xs ys. case_prod append (fold (\<lambda>x (ys, zs). (remove1 x ys, x # zs)) xs (ys, []))"
+    "op #" remove1 "\<lambda>L. mset (map mset L)" "op @" "\<lambda>L C. L \<in> set C" "op #"
+    remove_first
+    by unfold_locales (auto simp: ac_simps union_mset_list mset_map_mset_remove_first)
+end
+
+end
