Weidenbach_Book/CDCL_WNOT_Measure.thy
@@ -1,0 +1,187 @@
+theory CDCL_WNOT_Measure
+imports Main
+begin
+
+section \<open>Measure\<close>
+text \<open>This measure show the termination of the core of CDCL: each step improves the number of 
+  literals we know for sure.
+  
+  This measure can also be seen as the increasing lexicographic order: it is an order on bounded
+  sequences, when each element is bounded. The proof involves a measure like the one defined here
+  (the same?).\<close>
+definition \<mu>\<^sub>C  :: "nat \<Rightarrow> nat \<Rightarrow> nat list \<Rightarrow> nat" where
+"\<mu>\<^sub>C s b M \<equiv> (\<Sum>i=0..<length M. M!i * b^ (s +i - length M))"
+
+lemma \<mu>\<^sub>C_nil[simp]:
+  "\<mu>\<^sub>C s b [] = 0"
+  unfolding \<mu>\<^sub>C_def by auto
+
+lemma \<mu>\<^sub>C_single[simp]:
+  "\<mu>\<^sub>C s b [L] = L * b ^ (s - Suc 0)"
+  unfolding \<mu>\<^sub>C_def by auto
+
+lemma set_sum_atLeastLessThan_add:
+  "(\<Sum>i=k..<k+(b::nat). f i) = (\<Sum>i=0..<b. f (k+ i))"
+  by (induction b) auto
+
+lemma set_sum_atLeastLessThan_Suc:
+  "(\<Sum>i=1..<Suc j. f i) = (\<Sum>i=0..<j. f (Suc i))"
+  using set_sum_atLeastLessThan_add[of _ 1 j] by force
+
+lemma \<mu>\<^sub>C_cons:
+  "\<mu>\<^sub>C s b (L # M) = L * b ^ (s - 1 - length M) + \<mu>\<^sub>C s b M"
+proof -
+  have "\<mu>\<^sub>C s b (L # M) = (\<Sum>i=0..<length (L#M). (L#M)!i * b^ (s +i - length (L#M)))"
+    unfolding \<mu>\<^sub>C_def by blast
+  also have "\<dots> = (\<Sum>i=0..<1. (L#M)!i * b^ (s +i - length (L#M)))
+                 + (\<Sum>i=1..<length (L#M). (L#M)!i * b^ (s +i - length (L#M)))"
+     by (rule setsum_add_nat_ivl[symmetric]) simp_all
+  finally have "\<mu>\<^sub>C s b (L # M)= L * b ^ (s - 1 - length M)
+                  + (\<Sum>i=1..<length (L#M). (L#M)!i * b^ (s +i - length (L#M)))"
+     by auto
+  moreover {
+    have "(\<Sum>i=1..<length (L#M). (L#M)!i * b^ (s +i - length (L#M))) =
+           (\<Sum>i=0..<length (M). (L#M)!(Suc i) * b^ (s + (Suc i) - length (L#M)))"
+     unfolding length_Cons set_sum_atLeastLessThan_Suc by blast
+    also have "\<dots> = (\<Sum>i=0..<length (M). M!i * b^ (s + i - length M))"
+      by auto
+    finally have "(\<Sum>i=1..<length (L#M). (L#M)!i * b^ (s +i - length (L#M))) = \<mu>\<^sub>C s b M"
+      unfolding \<mu>\<^sub>C_def .
+    }
+  ultimately show ?thesis by presburger
+qed
+
+lemma \<mu>\<^sub>C_append:
+  assumes "s \<ge> length (M@M')"
+  shows "\<mu>\<^sub>C s b (M@M') = \<mu>\<^sub>C (s - length M') b M + \<mu>\<^sub>C s b M'"
+proof -
+  have "\<mu>\<^sub>C s b (M@M') = (\<Sum>i=0..<length (M@M'). (M@M')!i * b^ (s +i - length (M@M')))"
+    unfolding \<mu>\<^sub>C_def by blast
+  moreover then have "\<dots> = (\<Sum>i=0..< length M. (M@M')!i * b^ (s +i - length (M@M')))
+                 + (\<Sum>i=length M..<length (M@M'). (M@M')!i * b^ (s +i - length (M@M')))"
+    by (auto intro!: setsum_add_nat_ivl[symmetric])
+  moreover
+    have "\<forall>i\<in>{0..< length M}. (M@M')!i * b^ (s +i - length (M@M')) = M ! i * b ^ (s - length M'
+      + i - length M)"
+      using \<open>s \<ge> length (M@M')\<close> by (auto simp add: nth_append ac_simps)
+    then have "\<mu>\<^sub>C (s - length M') b M = (\<Sum>i=0..< length M. (M@M')!i * b^ (s +i - length (M@M')))"
+      unfolding \<mu>\<^sub>C_def by auto
+  ultimately have "\<mu>\<^sub>C s b (M@M')= \<mu>\<^sub>C (s - length M') b M
+                  + (\<Sum>i=length M..<length (M@M'). (M@M')!i * b^ (s +i - length (M@M')))"
+     by auto
+  moreover {
+    have "(\<Sum>i=length M..<length (M@M'). (M@M')!i * b^ (s +i - length (M@M'))) =
+           (\<Sum>i=0..<length M'. M'!i * b^ (s + i - length M'))"
+     unfolding length_append set_sum_atLeastLessThan_add by auto
+    then have "(\<Sum>i=length M..<length (M@M'). (M@M')!i * b^ (s +i - length (M@M'))) = \<mu>\<^sub>C s b M'"
+      unfolding \<mu>\<^sub>C_def .
+    }
+  ultimately show ?thesis by presburger
+qed
+
+lemma \<mu>\<^sub>C_cons_non_empty_inf:
+  assumes M_ge_1: "\<forall>i\<in>set M. i \<ge> 1" and M: "M \<noteq> []"
+  shows "\<mu>\<^sub>C s b M \<ge> b ^  (s - length M)"
+  using assms by (cases M) (auto simp: mult_eq_if \<mu>\<^sub>C_cons)
+
+text \<open>Duplicate of @{file "~~/src/HOL/ex/NatSum.thy"} (but generalized to @{term "k\<ge>0"})\<close>
+lemma sum_of_powers: "0 \<le> k \<Longrightarrow> (k - 1) * (\<Sum>i=0..<n. k^i) = k^n - (1::nat)"
+  apply (cases "k = 0")
+    apply (cases n; simp)
+  by (induct n) (auto simp: Nat.nat_distrib)
+
+text \<open>In the degenerated cases, we only have the large inequality holds. In the other cases, the
+  following strict inequality holds:\<close>
+lemma \<mu>\<^sub>C_bounded_non_degenerated:
+  fixes b ::nat
+  assumes
+    "b > 0" and
+    "M \<noteq> []" and
+    M_le: "\<forall>i < length M. M!i < b" and
+    "s \<ge> length M"
+  shows "\<mu>\<^sub>C s b M < b^s"
+proof -
+  consider (b1) "b= 1" | (b) "b>1" using \<open>b>0\<close> by (cases b) auto
+  then show ?thesis
+    proof cases
+      case b1
+      then have "\<forall>i < length M. M!i = 0" using M_le by auto
+      then have "\<mu>\<^sub>C s b M = 0" unfolding \<mu>\<^sub>C_def by auto
+      then show ?thesis using \<open>b > 0\<close> by auto
+    next
+      case b
+      have "\<forall> i \<in> {0..<length M}. M!i * b^ (s +i - length M) \<le> (b-1) * b^ (s +i - length M)"
+        using M_le \<open>b > 1\<close> by auto
+      then have "\<mu>\<^sub>C s b M \<le>  (\<Sum>i=0..<length M. (b-1) * b^ (s +i - length M))"
+         using \<open>M\<noteq>[]\<close> \<open>b>0\<close> unfolding \<mu>\<^sub>C_def by (auto intro: setsum_mono)
+      also
+        have "\<forall> i \<in> {0..<length M}. (b-1) * b^ (s +i - length M) = (b-1) * b^ i * b^(s - length M)"
+          by (metis Nat.add_diff_assoc2 add.commute assms(4) mult.assoc power_add)
+        then have "(\<Sum>i=0..<length M. (b-1) * b^ (s +i - length M))
+          = (\<Sum>i=0..<length M. (b-1)* b^ i * b^(s - length M))"
+          by (auto simp add: ac_simps)
+      also have "\<dots> = (\<Sum>i=0..<length M. b^ i) * b^(s - length M) * (b-1)"
+         by (simp add: setsum_left_distrib setsum_right_distrib ac_simps)
+      finally have "\<mu>\<^sub>C s b M \<le> (\<Sum>i=0..<length M. b^ i) * (b-1) * b^(s - length M)"
+        by (simp add: ac_simps)
+
+      also
+        have "(\<Sum>i=0..<length M. b^ i)* (b-1) = b ^ (length M) - 1"
+          using sum_of_powers[of b "length M"] \<open>b>1\<close>
+          by (auto simp add: ac_simps)
+      finally have "\<mu>\<^sub>C s b M \<le> (b ^ (length M) - 1) * b ^ (s - length M)"
+        by auto
+      also have "\<dots> < b ^ (length M) * b ^ (s - length M)"
+        using \<open>b>1\<close> by auto
+      also have "\<dots> = b ^ s"
+        by (metis assms(4) le_add_diff_inverse power_add)
+      finally show ?thesis unfolding \<mu>\<^sub>C_def by (auto simp add: ac_simps)
+    qed
+qed
+
+text \<open>In the degenerate case @{term "b=0"}, the list @{term M} is empty (since the list cannot
+  contain any element).\<close>
+lemma \<mu>\<^sub>C_bounded:
+  fixes b ::nat
+  assumes
+    M_le: "\<forall>i < length M. M!i < b" and
+    "s \<ge> length M"
+    "b > 0"
+  shows "\<mu>\<^sub>C s b M < b ^ s"
+proof -
+  consider (M0) "M = []" | (M) "b > 0" and "M \<noteq> []"
+    using M_le by (cases b, cases M) auto
+  then show ?thesis
+    proof cases
+      case M0
+      then show ?thesis using M_le \<open>b > 0\<close> by auto
+    next
+      case M
+      show ?thesis using \<mu>\<^sub>C_bounded_non_degenerated[OF M assms(1,2)] by arith
+    qed
+qed
+
+text \<open>When @{term "b=(0::nat)"}, we cannot show that the measure is empty, since @{term "0^0 =
+  (1::nat)"}.\<close>
+lemma \<mu>\<^sub>C_base_0:
+  assumes "length M \<le> s"
+  shows "\<mu>\<^sub>C s 0 M \<le> M!0"
+proof -
+  {
+    assume "s = length M"
+    moreover {
+      fix n
+      have "(\<Sum>i=0..<n. M ! i * (0::nat) ^ i) \<le> M ! 0"
+        apply (induction n rule: nat_induct)
+        by simp (rename_tac n, case_tac n, auto)
+    }
+    ultimately have ?thesis unfolding \<mu>\<^sub>C_def by auto
+  }
+  moreover
+  {
+    assume "length M < s"
+    then have "\<mu>\<^sub>C s 0 M = 0" unfolding \<mu>\<^sub>C_def by auto}
+  ultimately show ?thesis using assms unfolding \<mu>\<^sub>C_def by linarith
+qed
+
+end
